First part of labb2 done

Labb2/labb2.dfy
@@ -1,3 +1,5 @@
+// When you are finished,  all the below assertions should be provable.
+// Feel free to add extra ones as well.
 // A LIFO queue (aka a stack) with limited capacity.
 class LimitedStack{
 
@@ -6,38 +8,23 @@ class LimitedStack{
       var top : int; // The index of the top of the stack, or -1 if the stack is empty
 
       // This predicate express a class invariant: All objects of this calls should satisfy this.
-    predicate Valid() //arr : array<int>, top : int, capacity : int
-      //requires arr != null
-      reads this; // Does this mean it reads all the variables?
+    predicate Valid()
+      reads this;
       {
-        /*
-          arr != null &&
-          forall capacity : int :: capacity > 0 &&
-		      forall capacity : int :: arr.Length == capacity &&
-		      forall top : int, capacity : int :: top >= -1 && top < capacity
-        */
         arr != null && capacity > 0 && arr.Length == capacity
         && top >= -1 && top < capacity
       }
 
-      predicate Empty() //top : int
-      reads this; // Should this be "this"?
+      predicate Empty()
+      reads this;
       {
-        //forall top : int :: top == -1
         top == -1
       }
 
-      predicate method Full() //top : int, capacity : int
-      reads this; // Should this be "this"?
-      {
-        //forall top : int, capacity : int :: top == capacity - 1
-        top >= (capacity-1)
-      }
-
-      predicate NotFull()
+      predicate method Full()
       reads this;
       {
-        top != capacity -1
+        top >= (capacity-1)
       }
 
       method Init(c : int)
@@ -45,8 +32,8 @@ class LimitedStack{
         requires c > 0
         ensures fresh(arr); // ensures arr is a newly created object.
         // Additional post-condition to be given here!
-        ensures Valid(); //arr, top, c
-        ensures Empty() && capacity == c; //top
+        ensures Valid();
+        ensures Empty() && capacity == c;
         {
           capacity := c;
           arr := new int[c];
@@ -54,23 +41,16 @@ class LimitedStack{
       }
 
       method isEmpty() returns (res : bool)
-      //reads this.top;
       {
-        //var res : bool;
-        //^ måste tydligen inte deklarera variabler om de står som returns
-        //Får inte använda predicate i metoder, bara i specification
-        res := (top == -1); //top
+        res := (top == -1);
       }
-
-
 
       // Returns the top element of the stack, without removing it.
       method Peek() returns (elem : int)
-      //reads this.arr, this.top;
-      requires Valid() && !Empty(); //arr, top, capacity
+      requires Valid();
+      requires !Empty();
+      ensures elem == arr[top];
       {
-        //var elem : int;
-        //^ måste tydligen inte deklarera variabler om de står som returns
         elem := arr[top];
       }
 
@@ -78,40 +58,29 @@ class LimitedStack{
 
       // Pushed an element to the top of a (non full) stack.
       method Push(elem : int)
-      //reads this.arr, this.top, this.capacity;
-      //Should we put this as an ensures or in an if?
       modifies this`top, this.arr;
-      requires !Full(); //&& Valid();
-      //requires top != capacity - 1; //<-- this works for some reason
-      //requires NotFull();
-      requires Valid(); //top, capacity && arr, top, capacity
+      requires !Full() && Valid();
       ensures Valid() && !Empty() && arr[top] == elem && top == old(top) + 1;
-      //ensures Valid() && !Empty();
+      ensures forall i :: 0 <= i <= old(top) ==> arr[i] == old(arr[i]);
       {
-        //var booly := Full();
-        //print booly;
-       //if !Full(){ //or as an if
           top := top + 1;
           arr[top] := elem;
-        //}
       }
 
       // Pops the top element off the stack.
       method Pop() returns (elem : int)
-      //reads this.arr, this.top;
       modifies this`top, this.arr;
-      requires !Empty() && Valid(); //top && arr, top, capacity
-      ensures Valid() && top == old(top) - 1 && elem == old(arr[top]); //arr, top, capacity
+      requires !Empty() && Valid();
+      ensures Valid() && top == old(top) - 1 && elem == old(arr[top]);
+      ensures forall i :: 0 <= i < old(top) ==> arr[i] == old(arr[i]);
       {
-        //var elem : int;
         elem := arr[top];
         top := top - 1;
-        print top;
       }
 
       method Shift()
-      requires Valid() && !Empty() //arr, top, capacity && top
-      ensures Valid(); //arr, top, capacity
+      requires Valid() && !Empty()
+      ensures Valid();
       ensures forall i : int :: 0 <= i < capacity - 1 ==> arr[i] == old(arr[i + 1]);
       ensures top == old(top) - 1;
       modifies this.arr, this`top;
@@ -132,63 +101,48 @@ class LimitedStack{
 
       //Push onto full stack, oldest element is discarded.
       method Push2(elem : int)
-      //reads this.arr, this.top, this.capacity;
       modifies this.arr, this`top;
-      requires Valid(); //arr, top, capacity
-      ensures Valid() /*&& arr[top-1] == elem*/; //arr, top, capacity
+      requires Valid();
+      ensures Valid() && !Empty() && arr[top] == elem;
+      ensures forall i :: 0 <= i <= old(top) ==> arr[i] == old(arr[i])
+            || forall i :: 1 <= i <= old(top) ==> arr[i-1] == old(arr[i]);
       {
-        if Full() //top, capacity
+        if Full()
         {
           Shift();
         }
         Push(elem);
       }
 
-      //FOR TESTING
-      method getTop() returns (topRet : int)
-      {
-        topRet := top;
-      }
-
 
 // When you are finished,  all the below assertions should be provable.
 // Feel free to add extra ones as well.
       method Main(){
-           var s := new LimitedStack;
-           s.Init(3);
-                var whyyyyyyy := s.getTop();
-                print whyyyyyyy;
-           assert s.Empty() && !s.Full();
-                var why := s.getTop();
-                print why;
-           s.Push(27);
-           assert !s.Empty();
-                var fuckThisFuckingShit := s.getTop();
-                print fuckThisFuckingShit;
-           var e := s.Pop();
-           print e;
-           assert e == 27;
-                var p := s.getTop();
-                print p;
+        var s := new LimitedStack;
+        s.Init(3);
 
-           s.Push(5);
-           var p1 := s.getTop();
-           print p1;
- /*
-           s.Push(32);
-           s.Push(9);
-           assert s.Full();
+        assert s.Empty() && !s.Full();
 
-           var e2 := s.Pop();
-           assert e2 == 9 && !s.Full();
-           assert s.arr[0] == 5;
+        s.Push(27);
+        assert !s.Empty();
 
-           s.Push(e2);
-           s.Push2(99);
+        var e := s.Pop();
+        assert e == 27;
 
-           var e3 := s.Peek();
-           assert e3 == 99;
-           assert s.arr[0] == 32;
-           */
-       }
+        s.Push(5);
+        s.Push(32);
+        s.Push(9);
+        assert s.Full();
+
+        var e2 := s.Pop();
+        assert e2 == 9 && !s.Full();
+        assert s.arr[0] == 5;
+
+        s.Push(e2);
+        s.Push2(99);
+
+        var e3 := s.Peek();
+        assert e3 == 99;
+        assert s.arr[0] == 32;
+   }
 }
